tweak reader monad hoare logic notation

isabelle/Utils/Reader_Monad/Utils_Reader_Monad_Hoare.thy
@@ -8,68 +8,66 @@ begin
 
 definition hoare_triple ::
   \<open>['a \<Rightarrow> 'b \<Rightarrow> bool, 'b \<Rightarrow> ('a, 'c) reader_monad, 'a \<Rightarrow> 'c \<Rightarrow> bool] \<Rightarrow> bool\<close>
-  (\<open>\<turnstile> \<lbrace> _ \<rbrace> _ \<lbrace> _ \<rbrace> \<close> [21, 20, 21] 60) where
-  \<open>\<turnstile> \<lbrace>P\<rbrace> f \<lbrace>Q\<rbrace> \<equiv>
+  (\<open>\<turnstile>rd \<lbrakk> _ \<rbrakk> _ \<lbrakk> _ \<rbrakk> \<close> [21, 20, 21] 60) where
+  \<open>\<turnstile>rd \<lbrakk>P\<rbrakk> f \<lbrakk>Q\<rbrakk> \<equiv>
     \<forall> \<phi> x. P \<phi> x \<longrightarrow> Q \<phi> (run_reader (f x) \<phi>)\<close>
 
 lemma hoare_tripleI :
   assumes \<open>\<And> \<phi> x. P \<phi> x \<Longrightarrow> Q \<phi> (run_reader (f x) \<phi>)\<close>
-  shows \<open>\<turnstile> \<lbrace>P\<rbrace> f \<lbrace>Q\<rbrace>\<close>
+  shows \<open>\<turnstile>rd \<lbrakk>P\<rbrakk> f \<lbrakk>Q\<rbrakk>\<close>
   by (simp add: assms hoare_triple_def)
 
 lemma hoare_tripleE :
   assumes
-    \<open>\<turnstile> \<lbrace>P\<rbrace> f \<lbrace>Q\<rbrace>\<close>
+    \<open>\<turnstile>rd \<lbrakk>P\<rbrakk> f \<lbrakk>Q\<rbrakk>\<close>
     \<open>P \<phi> x\<close>
   shows \<open>Q \<phi> (run_reader (f x) \<phi>)\<close>
   by (metis assms hoare_triple_def)
 
 lemma precond_postcond :
   assumes
-    \<open>\<turnstile> \<lbrace>P\<rbrace> f \<lbrace>Q\<rbrace>\<close>
+    \<open>\<turnstile>rd \<lbrakk>P\<rbrakk> f \<lbrakk>Q\<rbrakk>\<close>
     \<open>\<And> \<phi> x. P' \<phi> x \<Longrightarrow> P \<phi> x\<close>
     \<open>\<And> \<phi> y. Q \<phi> y \<Longrightarrow> Q' \<phi> y\<close>
-  shows \<open>\<turnstile> \<lbrace>P'\<rbrace> f \<lbrace>Q'\<rbrace>\<close>
+  shows \<open>\<turnstile>rd \<lbrakk>P'\<rbrakk> f \<lbrakk>Q'\<rbrakk>\<close>
   by (metis assms hoare_tripleI hoare_tripleE)
 
 lemma postcond_true :
-  \<open>\<turnstile> \<lbrace>P\<rbrace> f \<lbrace>\<lblot>\<lblot>True\<rblot>\<rblot>\<rbrace>\<close>
+  \<open>\<turnstile>rd \<lbrakk>P\<rbrakk> f \<lbrakk>\<lblot>\<lblot>True\<rblot>\<rblot>\<rbrakk>\<close>
   by (simp add: hoare_tripleI)
 
 lemma get_rd :
-  fixes P
-  defines \<open>P' \<equiv> \<lambda> \<phi> _. P \<phi>\<close>
-  shows \<open>\<turnstile> \<lbrace>P'\<rbrace> \<lblot>get_rd\<rblot> \<lbrace>P'\<rbrace>\<close>
-  by (simp add: assms hoare_triple_def run_reader_simps)
+  \<open>\<turnstile>rd \<lbrakk>(\<lambda> \<phi>. \<lblot>P \<phi> \<phi>\<rblot>)\<rbrakk> \<lblot>get_rd\<rblot> \<lbrakk>P\<rbrakk>\<close>
+  by (simp add: hoare_triple_def run_reader_simps)
 
 lemma skip [simp] :
-  \<open>(\<turnstile> \<lbrace>P\<rbrace> return_rd \<lbrace>Q\<rbrace>) \<longleftrightarrow> (\<forall> \<phi> x. P \<phi> x \<longrightarrow> Q \<phi> x)\<close>
+  \<open>(\<turnstile>rd \<lbrakk>P\<rbrakk> return_rd \<lbrakk>Q\<rbrakk>) \<longleftrightarrow> (\<forall> \<phi> x. P \<phi> x \<longrightarrow> Q \<phi> x)\<close>
   by (simp add: hoare_triple_def run_reader_simps(1))
 
 lemma skip' [simp] :
-  \<open>(\<turnstile> \<lbrace>P\<rbrace> (\<lambda> x. return_rd (f x)) \<lbrace>Q\<rbrace>) \<longleftrightarrow> (\<forall> \<phi> x. P \<phi> x \<longrightarrow> Q \<phi> (f x))\<close>
+  \<open>(\<turnstile>rd \<lbrakk>P\<rbrakk> (\<lambda> x. return_rd (f x)) \<lbrakk>Q\<rbrakk>) \<longleftrightarrow> (\<forall> \<phi> x. P \<phi> x \<longrightarrow> Q \<phi> (f x))\<close>
   by (simp add: hoare_triple_def run_reader_simps(1))
 
 lemma if_then_else :
   assumes
-    \<open>\<And> b. f b \<Longrightarrow> \<turnstile> \<lbrace>P\<rbrace> g \<lbrace>Q\<rbrace>\<close>
-    \<open>\<And> b. \<not> f b \<Longrightarrow> \<turnstile> \<lbrace>P\<rbrace> h \<lbrace>Q\<rbrace>\<close>
-  shows \<open>\<turnstile> \<lbrace>P\<rbrace> (\<lambda> b. if f b then g b else h b) \<lbrace>Q\<rbrace>\<close>
+    \<open>\<And> b. f b \<Longrightarrow> \<turnstile>rd \<lbrakk>P\<rbrakk> g \<lbrakk>Q\<rbrakk>\<close>
+    \<open>\<And> b. \<not> f b \<Longrightarrow> \<turnstile>rd \<lbrakk>P\<rbrakk> h \<lbrakk>Q\<rbrakk>\<close>
+  shows \<open>\<turnstile>rd \<lbrakk>P\<rbrakk> (\<lambda> b. if f b then g b else h b) \<lbrakk>Q\<rbrakk>\<close>
   using assms by (simp add: hoare_triple_def)
 
 lemma seq :
   assumes
-    \<open>\<turnstile> \<lbrace>P\<rbrace> f \<lbrace>Q\<rbrace>\<close>
-    \<open>\<turnstile> \<lbrace>Q\<rbrace> g \<lbrace>R\<rbrace>\<close>
-  shows \<open>\<turnstile> \<lbrace>P\<rbrace> f >=> g \<lbrace>R\<rbrace>\<close>
+    \<open>\<turnstile>rd \<lbrakk>P\<rbrakk> f \<lbrakk>Q\<rbrakk>\<close>
+    \<open>\<turnstile>rd \<lbrakk>Q\<rbrakk> g \<lbrakk>R\<rbrakk>\<close>
+  shows \<open>\<turnstile>rd \<lbrakk>P\<rbrakk> f >=> g \<lbrakk>R\<rbrakk>\<close>
   using assms
   by (simp add: hoare_triple_def run_reader_simps(3))
 
 lemma seq' :
   assumes
-    \<open>\<turnstile> \<lbrace>P\<rbrace> f \<lbrace>Q\<rbrace>\<close>
-    \<open>\<And> \<phi> x. P \<phi> x \<Longrightarrow> \<turnstile> \<lbrace>Q\<rbrace> g x \<lbrace>R\<rbrace>\<close>
-  shows \<open>\<turnstile> \<lbrace>P\<rbrace> (\<lambda> x. (x |> (f >=> g x))) \<lbrace>R\<rbrace>\<close>
+    \<open>\<turnstile>rd \<lbrakk>P\<rbrakk> f \<lbrakk>Q\<rbrakk>\<close>
+    \<open>\<And> \<phi> x. P \<phi> x \<Longrightarrow> \<turnstile>rd \<lbrakk>Q\<rbrakk> g x \<lbrakk>R\<rbrakk>\<close>
+  shows \<open>\<turnstile>rd \<lbrakk>P\<rbrakk> (\<lambda> x. (x |> (f >=> g x))) \<lbrakk>R\<rbrakk>\<close>
   using assms by (simp add: hoare_triple_def run_reader_simps(3))
 
 context
@@ -83,10 +81,10 @@ abbreviation (input)
   \<open>P' index \<phi> val \<equiv> index < offset + length xs \<and> P index \<phi> val\<close>
 
 lemma loop_enumerate :
-  \<open>(\<And> index x. \<turnstile> \<lbrace>P' index\<rbrace> f (index, x) \<lbrace>P (Suc index)\<rbrace>)
-    \<Longrightarrow> \<turnstile> \<lbrace>P offset\<rbrace>
-          foldM_rd_enumerate f xs offset
-          \<lbrace>P (offset + length xs)\<rbrace>\<close>
+  \<open>(\<And> index x. \<turnstile>rd \<lbrakk>P' index\<rbrakk> f (index, x) \<lbrakk>P (Suc index)\<rbrakk>) \<Longrightarrow>
+  \<turnstile>rd \<lbrakk>P offset\<rbrakk>
+      foldM_rd_enumerate f xs offset
+      \<lbrakk>P (offset + length xs)\<rbrakk>\<close>
 proof (induction xs arbitrary: offset)
   case Nil
   then show ?case by (simp add: foldM_enumerate_def)
@@ -101,8 +99,8 @@ next
 qed
 
 lemma loop :
-  assumes \<open>\<And> index x. \<turnstile> \<lbrace>P' index\<rbrace> f x \<lbrace>P (Suc index)\<rbrace>\<close>
-  shows \<open>\<turnstile> \<lbrace>P offset\<rbrace> foldM_rd f xs \<lbrace>P (offset + length xs)\<rbrace>\<close>
+  assumes \<open>\<And> index x. \<turnstile>rd \<lbrakk>P' index\<rbrakk> f x \<lbrakk>P (Suc index)\<rbrakk>\<close>
+  shows \<open>\<turnstile>rd \<lbrakk>P offset\<rbrakk> foldM_rd f xs \<lbrakk>P (offset + length xs)\<rbrakk>\<close>
   using assms
   by (auto
     intro: loop_enumerate
@@ -111,8 +109,8 @@ lemma loop :
 end
 
 lemma loop_unindexed :
-  assumes \<open>\<And> x. \<turnstile> \<lbrace>P\<rbrace> f x \<lbrace>P\<rbrace>\<close>
-  shows \<open>\<turnstile> \<lbrace>P\<rbrace> foldM_rd f xs \<lbrace>P\<rbrace>\<close>
+  assumes \<open>\<And> x. \<turnstile>rd \<lbrakk>P\<rbrakk> f x \<lbrakk>P\<rbrakk>\<close>
+  shows \<open>\<turnstile>rd \<lbrakk>P\<rbrakk> foldM_rd f xs \<lbrakk>P\<rbrakk>\<close>
   using loop[where ?P = \<open>curry <| snd >>> P\<close>, where ?offset = 0] assms
   by (fastforce simp add: hoare_triple_def curry_def snd_def)
 
