isabelle/Utils/Reader_Monad/Utils_Reader_Monad_Relational.thy
@@ -11,46 +11,49 @@ definition
     R \<phi> (run_reader m \<phi>) \<phi>' (run_reader m' \<phi>')\<close>
 
 definition relational_hoare_triple
-  (\<open>\<turnstile> \<lbrace> _ \<rbrace> \<langle> _ | _ \<rangle> \<lbrace> _ \<rbrace>\<close> [21, 20, 20, 21] 60) where
-  \<open>(\<turnstile> \<lbrace>R\<rbrace> \<langle>f | f'\<rangle> \<lbrace>S\<rbrace>) \<equiv>
+  (\<open>\<turnstile>rd \<lbrakk> _ \<rbrakk> \<langle> _ | _ \<rangle> \<lbrakk> _ \<rbrakk>\<close> [21, 20, 20, 21] 60) where
+  \<open>(\<turnstile>rd \<lbrakk>R\<rbrakk> \<langle>f | f'\<rangle> \<lbrakk>S\<rbrakk>) \<equiv>
     \<forall> \<phi> x \<phi>' x'. R \<phi> x \<phi>' x' \<longrightarrow> rel_rd S \<phi> (f x) \<phi>' (f' x')\<close>
 
 lemma relational_hoare_iff_hoare [simp] :
-  \<open>(\<turnstile> \<lbrace>(\<lambda> \<phi> x \<phi>' x'. R \<phi> x \<and> R \<phi>' x')\<rbrace>
+  \<open>(\<turnstile>rd \<lbrakk>(\<lambda> \<phi> x \<phi>' x'. R \<phi> x \<and> R \<phi>' x')\<rbrakk>
     \<langle>f | f\<rangle>
-    \<lbrace>(\<lambda> \<phi> x \<phi>' x'. S \<phi> x \<and> S \<phi>' x')\<rbrace>)
-  \<longleftrightarrow> (\<turnstile> \<lbrace>R\<rbrace> f \<lbrace>S\<rbrace>)\<close>
+    \<lbrakk>(\<lambda> \<phi> x \<phi>' x'. S \<phi> x \<and> S \<phi>' x')\<rbrakk>)
+  \<longleftrightarrow> (\<turnstile>rd \<lbrakk>R\<rbrakk> f \<lbrakk>S\<rbrakk>)\<close>
   by (smt (verit, best) hoare_triple_def rel_rd_def relational_hoare_triple_def)
 
-lemma skip_left [simp] :
-  \<open>(\<turnstile> \<lbrace>(\<lambda> \<phi> x \<phi>' x'. R \<phi> x \<phi>' x')\<rbrace>
-    \<langle>return_rd | f\<rangle>
-    \<lbrace>(\<lambda> \<phi> x \<phi>' x'. S \<phi> x \<phi>' x')\<rbrace>)
-  \<longleftrightarrow> (\<forall> \<phi> x. \<turnstile> \<lbrace>R \<phi> x\<rbrace> f \<lbrace>S \<phi> x\<rbrace>)\<close>
-  by (smt (verit) hoare_triple_def rel_rd_def relational_hoare_triple_def run_reader_simps(1))
-
 lemma skip [simp] :
-  \<open>\<turnstile> \<lbrace>R\<rbrace> \<langle>return_rd | return_rd\<rangle> \<lbrace>S\<rbrace>
+  \<open>\<turnstile>rd \<lbrakk>R\<rbrakk> \<langle>return_rd | return_rd\<rangle> \<lbrakk>S\<rbrakk>
   \<longleftrightarrow> (\<forall> \<phi> x \<phi>' x'. R \<phi> x \<phi>' x' \<longrightarrow> S \<phi> x \<phi>' x')\<close>
-  by (simp add: relational_hoare_triple_def rel_rd_def run_reader_simps(1))
+
+  \<open>(\<turnstile>rd \<lbrakk>(\<lambda> \<phi> x \<phi>' x'. R \<phi> x \<phi>' x')\<rbrakk>
+    \<langle>return_rd | f\<rangle>
+    \<lbrakk>(\<lambda> \<phi> x \<phi>' x'. S \<phi> x \<phi>' x')\<rbrakk>)
+  \<longleftrightarrow> (\<forall> \<phi> x. \<turnstile>rd \<lbrakk>R \<phi> x\<rbrakk> f \<lbrakk>S \<phi> x\<rbrakk>)\<close>
+
+  \<open>(\<turnstile>rd \<lbrakk>(\<lambda> \<phi> x \<phi>' x'. R \<phi> x \<phi>' x')\<rbrakk>
+    \<langle>f | return_rd\<rangle>
+    \<lbrakk>(\<lambda> \<phi> x \<phi>' x'. S \<phi> x \<phi>' x')\<rbrakk>)
+  \<longleftrightarrow> (\<forall> \<phi>' x'. \<turnstile>rd \<lbrakk>(\<lambda> \<phi> x. R \<phi> x \<phi>' x')\<rbrakk> f \<lbrakk>(\<lambda> \<phi> x. S \<phi> x \<phi>' x')\<rbrakk>)\<close>
+  by (auto simp add: relational_hoare_triple_def hoare_triple_def rel_rd_def run_reader_simps(1))
 
 lemma skip' [simp] :
-  \<open>\<turnstile> \<lbrace>R\<rbrace> \<langle>(\<lambda> x. return_rd (f x)) | (\<lambda> x. return_rd (f' x))\<rangle> \<lbrace>S\<rbrace>
+  \<open>\<turnstile>rd \<lbrakk>R\<rbrakk> \<langle>(\<lambda> x. return_rd (f x)) | (\<lambda> x. return_rd (f' x))\<rangle> \<lbrakk>S\<rbrakk>
   \<longleftrightarrow> (\<forall> \<phi> x \<phi>' x'. R \<phi> x \<phi>' x' \<longrightarrow> S \<phi> (f x) \<phi>' (f' x'))\<close>
   by (simp add: relational_hoare_triple_def rel_rd_def run_reader_simps(1))
 
 lemma seq :
   assumes
-    \<open>\<turnstile> \<lbrace>R\<rbrace> \<langle>f | f'\<rangle> \<lbrace>S\<rbrace>\<close>
-    \<open>\<turnstile> \<lbrace>S\<rbrace> \<langle>g | g'\<rangle> \<lbrace>T\<rbrace>\<close>
-  shows \<open>\<turnstile> \<lbrace>R\<rbrace> \<langle>(f >=> g) | (f' >=> g')\<rangle> \<lbrace>T\<rbrace>\<close>
+    \<open>\<turnstile>rd \<lbrakk>R\<rbrakk> \<langle>f | f'\<rangle> \<lbrakk>S\<rbrakk>\<close>
+    \<open>\<turnstile>rd \<lbrakk>S\<rbrakk> \<langle>g | g'\<rangle> \<lbrakk>T\<rbrakk>\<close>
+  shows \<open>\<turnstile>rd \<lbrakk>R\<rbrakk> \<langle>f >=> g | f' >=> g'\<rangle> \<lbrakk>T\<rbrakk>\<close>
   using assms by (simp add: rel_rd_def relational_hoare_triple_def run_reader_simps(3))
 
 lemma seq' :
   assumes
-    \<open>\<turnstile> \<lbrace>R\<rbrace> \<langle>f | f'\<rangle> \<lbrace>S\<rbrace>\<close>
-    \<open>\<And> \<phi> x \<phi>' x'. R \<phi> x \<phi>' x' \<Longrightarrow> \<turnstile> \<lbrace>S\<rbrace> \<langle>g x | g' x'\<rangle> \<lbrace>T\<rbrace>\<close>
-  shows \<open>\<turnstile> \<lbrace>R\<rbrace> \<langle>(\<lambda> x. (x |> (f >=> g x))) | (\<lambda> x. (x |> (f' >=> g' x)))\<rangle> \<lbrace>T\<rbrace>\<close>
+    \<open>\<turnstile>rd \<lbrakk>R\<rbrakk> \<langle>f | f'\<rangle> \<lbrakk>S\<rbrakk>\<close>
+    \<open>\<And> \<phi> x \<phi>' x'. R \<phi> x \<phi>' x' \<Longrightarrow> \<turnstile>rd \<lbrakk>S\<rbrakk> \<langle>g x | g' x'\<rangle> \<lbrakk>T\<rbrakk>\<close>
+  shows \<open>\<turnstile>rd \<lbrakk>R\<rbrakk> \<langle>(\<lambda> x. (x |> (f >=> g x))) | (\<lambda> x. (x |> (f' >=> g' x)))\<rangle> \<lbrakk>T\<rbrakk>\<close>
   using assms by (simp add: rel_rd_def relational_hoare_triple_def run_reader_simps(3))
 
 context
@@ -67,10 +70,10 @@ abbreviation (input)
   \<open>R' index \<phi> val \<phi>' val' \<equiv> index < offset + length xs \<and> R index \<phi> val \<phi>' val'\<close>
 
 lemma loop_enumerate :
-  \<open>(\<And> index x. \<turnstile> \<lbrace>R' index\<rbrace> \<langle>f (index, x) | f' (index, x)\<rangle> \<lbrace>R (Suc index)\<rbrace>)
-    \<Longrightarrow> \<turnstile> \<lbrace>R offset\<rbrace>
-        \<langle>foldM_enumerate' f | foldM_enumerate' f'\<rangle>
-        \<lbrace>R (offset + length xs)\<rbrace>\<close>
+  \<open>(\<And> index x. \<turnstile>rd \<lbrakk>R' index\<rbrakk> \<langle>f (index, x) | f' (index, x)\<rangle> \<lbrakk>R (Suc index)\<rbrakk>) \<Longrightarrow>
+  \<turnstile>rd \<lbrakk>R offset\<rbrakk>
+      \<langle>foldM_enumerate' f | foldM_enumerate' f'\<rangle>
+      \<lbrakk>R (offset + length xs)\<rbrakk>\<close>
 proof (induction xs arbitrary: offset)
   case Nil
   then show ?case by (simp add: foldM_enumerate_def)
@@ -85,11 +88,11 @@ next
 qed
 
 lemma loop :
-  assumes \<open>\<And> index x. \<turnstile> \<lbrace>R' index\<rbrace> \<langle>f x | f' x\<rangle> \<lbrace>R (Suc index)\<rbrace>\<close>
-  shows
-    \<open>\<turnstile> \<lbrace>R offset\<rbrace>
-      \<langle>foldM_rd f xs | foldM_rd f' xs\<rangle>
-      \<lbrace>R (offset + length xs)\<rbrace>\<close>
+  assumes \<open>\<And> index x. \<turnstile>rd \<lbrakk>R' index\<rbrakk> \<langle>f x | f' x\<rangle> \<lbrakk>R (Suc index)\<rbrakk>\<close>
+  shows \<open>\<turnstile>rd
+    \<lbrakk>R offset\<rbrakk>
+    \<langle>foldM_rd f xs | foldM_rd f' xs\<rangle>
+    \<lbrakk>R (offset + length xs)\<rbrakk>\<close>
   using assms
   by (auto
     intro: loop_enumerate
@@ -98,8 +101,8 @@ lemma loop :
 end
 
 lemma loop_unindexed :
-  assumes \<open>\<And> x. \<turnstile> \<lbrace>R\<rbrace> \<langle>f x | f' x\<rangle> \<lbrace>R\<rbrace>\<close>
-  shows \<open>\<turnstile> \<lbrace>R\<rbrace> \<langle>foldM_rd f xs | foldM_rd f' xs\<rangle> \<lbrace>R\<rbrace>\<close>
+  assumes \<open>\<And> x. \<turnstile>rd \<lbrakk>R\<rbrakk> \<langle>f x | f' x\<rangle> \<lbrakk>R\<rbrakk>\<close>
+  shows \<open>\<turnstile>rd \<lbrakk>R\<rbrakk> \<langle>foldM_rd f xs | foldM_rd f' xs\<rangle> \<lbrakk>R\<rbrakk>\<close>
   using loop[where ?R = \<open>\<lambda> _ x. R x\<close>, where ?offset = 0] assms
   by (fastforce simp add: relational_hoare_triple_def curry_def snd_def)
 
